WIP Rust nondet snapshot

src/cbor/pulse/nondet/rust/src/lib.rs
@@ -1,0 +1,16 @@
+#[macro_use]
+extern crate static_assertions;
+
+const_assert!(usize::BITS >= 64);
+
+mod lowstar {
+    pub mod ignore {
+        pub fn ignore<T>(_: T) {}
+    }
+}
+
+mod cbornondetveraux;
+
+pub mod cbornondetver;
+
+pub mod cbornondet;
