src/cbor/pulse/nondet/rust/tests/example.rs
@@ -1,0 +1,81 @@
+use cborrs::cbornondet::*;
+use cborrs::cbornondet::CborNondetIntKind::*;
+use cborrs::cbornondet::CborNondetView::*;
+
+#[test]
+fn test()
+{
+    // Constructs 3 map entries: ("foo" -> 18), ("bar" -> -1-42), (1729 -> "quux")
+    let mut map_entries : [CborNondetMapEntry; 3] =
+        [
+            cbor_nondet_mk_map_entry(cbor_nondet_mk_text_string("foo").unwrap(), cbor_nondet_mk_int64(UInt64, 18)),
+            cbor_nondet_mk_map_entry(cbor_nondet_mk_text_string("bar").unwrap(), cbor_nondet_mk_int64(NegInt64, 42)),
+            cbor_nondet_mk_map_entry(cbor_nondet_mk_int64(UInt64, 1729), cbor_nondet_mk_text_string("quux").unwrap()),
+        ];
+
+    // Constructs an integer object to be used as the payload of a tagged object
+    let myint = cbor_nondet_mk_int64(UInt64, 2);
+
+    // Constructs 3 elements, in this order:
+    // - the integer object `myint`, tagged with 1234
+    // - a byte string
+    // - the map whose entries are defined in `map_entries` above
+    let array_entries : [CborNondet; 3] =
+        [
+            cbor_nondet_mk_tagged(1234, & myint),
+            cbor_nondet_mk_byte_string(& [18, 42, 17, 29]).unwrap(),
+            cbor_nondet_mk_map(& mut map_entries).unwrap()
+        ];
+
+    // Constructs an array object whose entries are defined
+    // in `array_entries` above
+    let test = cbor_nondet_mk_array(&array_entries).unwrap();
+
+    // Test reading from the just-constructed object
+    test_on(test);
+
+    // Allocate an output array to serialize our object
+    const max_size: usize = 32;
+    let mut output_bytes : [u8; max_size] = [0xFF; max_size];
+
+    // Now let's try to serialize our object into a small slice of the
+    // output array. It should fail
+    assert!(cbor_nondet_serialize(test, & mut output_bytes[0..16]) == None);
+
+    // Now serialize our object into the whole output array (we chose
+    // `max_size` to be large enough beforehand)
+    let size = cbor_nondet_serialize(test, & mut output_bytes).unwrap();
+
+    // Then, parse our object from the output array, and test reading
+    // from it
+    let (read, rem) = cbor_nondet_parse(&output_bytes).unwrap();
+    assert!(max_size - rem.len () == size);
+    test_on(read);
+
+    // Then, parse our object from only the written slice of the
+    // output array, and test reading from it
+    let (read, rem) = cbor_nondet_parse(&output_bytes[0..size]).unwrap();
+    assert!(rem.len () == 0);
+    test_on(read);
+}
+
+/// A test function to walk through the CBOR object we constructed in
+/// `test`. It will be called first with the `test` object as
+/// constructed, then with a serialization of this object.
+fn test_on(test: CborNondet)
+{
+    // Destruct the just constructed array and check its length
+    let Array { _0: a } = cbor_nondet_destruct(test) else { panic!("Array expected!"); };
+    assert!(cbor_nondet_get_array_length(a) == 3);
+
+    // Get the map, as the array element at index 2
+    let mymap = cbor_nondet_get_array_item(a, 2).unwrap();
+    let Map { _0: m } = cbor_nondet_destruct(mymap) else { panic!("Map expected!"); };
+
+    // Check the map value associated to "bar"
+    let bar_value = cbor_nondet_map_get(m, cbor_nondet_mk_text_string("bar").unwrap()).unwrap();
+    assert!(cbor_nondet_destruct(bar_value) == Int64 { kind: NegInt64, value: 42 });
+
+    // Alternatively, check with the cbornondet equality comparison
+    assert!(cbor_nondet_equal(bar_value, cbor_nondet_mk_int64(NegInt64, 42)));
+}
