src/cbor/pulse/raw/CBOR.Pulse.API.Nondet.C.fst
@@ -87,15 +87,15 @@ let cbor_nondet_map_entry_gather () = Rust.cbor_nondet_map_entry_gather ()
 
 let cbor_nondet_equal x1 #p1 #v1 x2 #p2 #v2 = Rust.cbor_nondet_equal x1 #p1 #v1 x2 #p2 #v2
 
-let cbor_nondet_map_get () = map_get_by_ref_safe (cbor_nondet_major_type ()) (Rust.cbor_nondet_map_get ())
+let cbor_nondet_map_get () = map_get_by_ref_safe (cbor_nondet_major_type ()) (map_get_as_ref (Rust.cbor_nondet_map_get ()))
 
 let cbor_nondet_mk_simple_value () = mk_simple_safe (Rust.cbor_nondet_mk_simple_value ())
 
-let cbor_nondet_mk_uint64 () v = Rust.cbor_nondet_mk_int64 () cbor_major_type_uint64 v
+let cbor_nondet_mk_uint64 () v = Rust.cbor_nondet_mk_uint64 () v
 
-let cbor_nondet_mk_neg_int64 () v = Rust.cbor_nondet_mk_int64 () cbor_major_type_neg_int64 v
+let cbor_nondet_mk_neg_int64 () v = Rust.cbor_nondet_mk_neg_int64 () v
 
-let cbor_nondet_mk_int64 () = mk_signed_int64 (Rust.cbor_nondet_mk_int64 ())
+let cbor_nondet_mk_int64 () v = Rust.cbor_nondet_mk_int64 () v
 
 let cbor_nondet_mk_byte_string () = mk_string_from_arrayptr (Rust.cbor_nondet_mk_string ()) cbor_major_type_byte_string
 
@@ -107,6 +107,263 @@ let cbor_nondet_mk_array () = mk_array_from_arrayptr (Rust.cbor_nondet_mk_array 
 
 let cbor_nondet_mk_map_entry () xk xv #pk #vk #pv #vv = Rust.cbor_nondet_mk_map_entry () xk xv #pk #vk #pv #vv
 
-let cbor_nondet_mk_map () = cbor_mk_map_from_arrayptr_safe (Rust.cbor_nondet_mk_map_gen ())
+let cbor_nondet_mk_map () = cbor_mk_map_from_arrayptr_safe (mk_map_gen_by_ref (Rust.cbor_nondet_mk_map ()))
+
+
+noextract [@noextract_to "krml"]
+let set_snd_None
+  (t1 t2: Type)
+  (x: (t1 & option t2))
+: Tot (t1 & option t2)
+= (fst x, None)
+
+module PM = Pulse.Lib.SeqMatch.Util
+
+ghost fn trade_assoc_hyp_r2l
+  (a b c d: slprop)
+requires
+  Trade.trade (a ** (b ** c)) d
+ensures
+  Trade.trade ((a ** b) ** c) d
+{
+  slprop_equivs ();
+  rewrite Trade.trade (a ** (b ** c)) d as Trade.trade ((a ** b) ** c) d
+}
+
+ghost fn trade_assoc_hyp_l2r
+  (a b c d: slprop)
+requires
+  Trade.trade ((a ** b) ** c) d
+ensures
+  Trade.trade (a ** (b ** c)) d
+{
+  slprop_equivs ();
+  rewrite Trade.trade ((a ** b) ** c) d as Trade.trade (a ** (b ** c)) d
+}
+
+ghost fn trade_assoc_concl_r2l
+  (a b c d: slprop)
+requires
+  Trade.trade a (b ** (c ** d))
+ensures
+  Trade.trade a ((b ** c) ** d)
+{
+  slprop_equivs ();
+  rewrite Trade.trade a (b ** (c ** d)) as Trade.trade a ((b ** c) ** d)
+}
+
+ghost fn trade_assoc_concl_l2r
+  (a b c d: slprop)
+requires
+  Trade.trade a ((b ** c) ** d)
+ensures
+  Trade.trade a (b ** (c ** d))
+{
+  slprop_equivs ();
+  rewrite Trade.trade a ((b ** c) ** d) as Trade.trade a (b ** (c ** d))
+}
+
+let list_memP_map_intro_forall
+  (#a #b: Type)
+  (f: a -> Tot b)
+  (l: list a)
+: Lemma
+  (requires True)
+  (ensures (forall x . List.Tot.memP x l ==> List.Tot.memP (f x) (List.Tot.map f l)))
+= let prf
+    (x: a)
+  : Lemma
+    (ensures List.Tot.memP x l ==> List.Tot.memP (f x) (List.Tot.map f l))
+  = List.Tot.memP_map_intro f x l
+  in
+  Classical.forall_intro prf
+
+ghost fn lemma_trade_ab_cd_e
+  (a b1 b2 c d1 d2 e: slprop)
+requires
+  Trade.trade (b1 ** d1) (b2 ** d2) **
+  Trade.trade ((a ** b2) ** (c ** d2)) e
+ensures
+  Trade.trade ((a ** b1) ** (c ** d1)) e
+{
+  slprop_equivs ();
+  rewrite (Trade.trade ((a ** b2) ** (c ** d2)) e) as Trade.trade ((a ** c) ** (b2 ** d2)) e;
+  Trade.trans_hyp_r (a ** c) _ _ _;
+  rewrite Trade.trade ((a ** c) ** (b1 ** d1)) e as (Trade.trade ((a ** b1) ** (c ** d1)) e)
+}
+
+ghost fn trade_prod_cancel_hyp_r_concl_l
+  (#a b #c #d #e: slprop)
+requires
+  Trade.trade (a ** b) c ** Trade.trade d (b ** e)
+ensures
+  Trade.trade (a ** d) (c ** e)
+{
+  intro
+    (Trade.trade (a ** d) (c ** e))
+    #(Trade.trade (a ** b) c ** Trade.trade d (b ** e))
+    fn _ {
+      Trade.elim d _;
+      Trade.elim (a ** b) _
+    }
+}
+
+ghost fn trade_prod_cancel_hyp_l_concl_l
+  (b #a #c #d #e: slprop)
+requires
+  Trade.trade (b ** a) c ** Trade.trade d (b ** e)
+ensures
+  Trade.trade (a ** d) (c ** e)
+{
+  slprop_equivs ();
+  rewrite Trade.trade (b ** a) c as Trade.trade (a ** b) c;
+  trade_prod_cancel_hyp_r_concl_l b
+}
+
+ghost fn trade_prod_cancel_hyp_r_concl_r
+  (#a b #c #d #e: slprop)
+requires
+  Trade.trade (a ** b) c ** Trade.trade d (e ** b)
+ensures
+  Trade.trade (a ** d) (c ** e)
+{
+  slprop_equivs ();
+  rewrite Trade.trade d (e ** b) as Trade.trade d (b ** e);
+  trade_prod_cancel_hyp_r_concl_l b
+}
+
+ghost fn trade_prod_cancel_hyp_l_concl_r
+  (b #a #c #d #e: slprop)
+requires
+  Trade.trade (b ** a) c ** Trade.trade d (e ** b)
+ensures
+  Trade.trade (a ** d) (c ** e)
+{
+  slprop_equivs ();
+  rewrite Trade.trade (b ** a) c as Trade.trade (a ** b) c;
+  trade_prod_cancel_hyp_r_concl_r b;
+}
+
+ghost fn trade_prod_cancel_concl_r_hyp_l
+  (#a #b c #d #e: slprop)
+requires
+  Trade.trade a (b ** c) ** Trade.trade (c ** d) e
+ensures
+  Trade.trade (a ** d) (b ** e)
+{
+  slprop_equivs ();
+  rewrite Trade.trade (c ** d) e as Trade.trade (d ** c) e;
+  trade_prod_cancel_hyp_r_concl_r c;
+  rewrite Trade.trade (d ** a) (e ** b) as Trade.trade (a ** d) (b ** e)
+}
+
+ghost fn trade_prod_cancel_concl_l_hyp_l
+  (#a c #b #d #e: slprop)
+requires
+  Trade.trade a (c ** b) ** Trade.trade (c ** d) e
+ensures
+  Trade.trade (a ** d) (b ** e)
+{
+  slprop_equivs ();
+  rewrite Trade.trade a (c ** b) as Trade.trade a (b ** c);
+  trade_prod_cancel_concl_r_hyp_l c;
+}
+
+ghost fn trade_prod_cancel_concl_r_hyp_r
+  (#a #b c #d #e: slprop)
+requires
+  Trade.trade a (b ** c) ** Trade.trade (d ** c) e
+ensures
+  Trade.trade (a ** d) (b ** e)
+{
+  slprop_equivs ();
+  rewrite Trade.trade (d ** c) e as Trade.trade (c ** d) e;
+  trade_prod_cancel_concl_r_hyp_l c
+}
+
+ghost fn trade_prod_cancel_concl_l_hyp_r
+  (#a c #b #d #e: slprop)
+requires
+  Trade.trade a (c ** b) ** Trade.trade (d ** c) e
+ensures
+  Trade.trade (a ** d) (b ** e)
+{
+  slprop_equivs ();
+  rewrite Trade.trade a (c ** b) as Trade.trade a (b ** c);
+  trade_prod_cancel_concl_r_hyp_r c
+}
+
+ghost fn trade_comm_concl
+  (a b c: slprop)
+requires Trade.trade a (b ** c)
+ensures Trade.trade a (c ** b)
+{
+  slprop_equivs();
+  rewrite Trade.trade a (b ** c) as Trade.trade a (c ** b)
+}
+
+let lemma_seq_assoc_cons
+  (#t: Type)
+  (a: Seq.seq t)
+  (b: t)
+  (c: Seq.seq t)
+: Lemma
+  (Seq.equal (Seq.append a (Seq.cons b c)) (Seq.append (Seq.append a (Seq.cons b Seq.empty)) c))
+= ()
+
+let lemma_seq_assoc_cons_upd
+  (#t: Type)
+  (a: Seq.seq t)
+  (c: Seq.seq t)
+  (b': t)
+: Lemma
+  (requires Seq.length c > 0)
+  (ensures Seq.equal
+    (Seq.upd (Seq.append a c) (Seq.length a) b')
+    (Seq.append (Seq.append a (Seq.cons b' Seq.empty)) (Seq.tail c))
+  )
+= ()
+
+ghost fn lemma_trade_rewrite5
+  (a b c d ef: slprop)
+requires
+   Trade.trade (((a **
+        b) **
+        c) **
+        d)
+      (ef)
+ensures
+   Trade.trade (a ** (d ** b ** c))
+      (ef)
+{
+  slprop_equivs ();
+  rewrite
+   Trade.trade (((a **
+        b) **
+        c) **
+        d)
+      (ef)
+  as Trade.trade (a ** (d ** b ** c))
+      (ef)
+}
+
+ghost fn cbor_map_get_multiple_entry_match_snd_prop
+  (#t: Type0)
+  (vmatch: perm -> t -> Spec.cbor -> slprop)
+  (x: cbor_map_get_multiple_entry_t t)
+  (y: option Spec.cbor)
+requires
+  cbor_map_get_multiple_entry_match_snd vmatch true x y
+ensures
+  cbor_map_get_multiple_entry_match_snd vmatch true x y **
+  pure (x.found == Some? y)
+{
+  if (x.found <> Some? y) {
+    rewrite cbor_map_get_multiple_entry_match_snd vmatch true x y as pure False;
+    rewrite emp as cbor_map_get_multiple_entry_match_snd vmatch true x y
+  }
+}
+
+module S = Pulse.Lib.Slice.Util
 
 let cbor_nondet_map_get_multiple () = cbor_map_get_multiple_as_arrayptr cbor_nondet_map_get_multiple_entry_t (cbor_nondet_major_type ()) (Rust.cbor_nondet_map_get_multiple ())
